CertiGC/cc_bitwise_encoding.v
@@ -2,42 +2,51 @@ Require Import RamifyCoq.CertiGC.bitwise_encoding.
 Require Import VST.floyd.proofauto.
 
 Class tagint_lossless {A : Type} (tcA : tagcode A) : Type :=
-  til_bound: (tc_bitsize tcA <= Int.wordsize)%nat.
+  til_bound: (tag_bitsize tcA <= Int.wordsize)%nat.
 
-Definition int_of_tag {A : Type} `{tcA : tagcode A} : A -> int :=
-  fun a => Int.repr (tc_encode tcA a).
+Definition int_of_tag {A : Type} `{tcA : tagcode A} : A -> int:=
+  fun a => Int.repr (tag_encode tcA a).
 
 Definition tag_of_int {A : Type} `{tcA : tagcode A} : int -> A :=
-  fun i => tc_decode tcA (Int.unsigned i).
+  fun i => tag_decode tcA (Int.unsigned i).
 
 Lemma tag_of_int_of_tag {A} `{tcA : tagcode A} `{tcAl: @tagint_lossless A tcA}: forall a,
   tag_of_int (int_of_tag a) = a.
 Proof.
   intros.
   red in tcAl. unfold tag_of_int, int_of_tag.
-  rewrite Int.unsigned_repr. apply tc_decode_encode.
-  generalize (tc_encode_range tcA a); intro.
+  rewrite Int.unsigned_repr. apply tag_decode_encode.
+  generalize (tag_encode_range tcA a); intro.
   unfold Int.max_unsigned. unfold Int.modulus.
   apply two_power_nat_le in tcAl.
   omega.
 Qed.
 
 Lemma int_of_tag_modu {A} {B} `{tcA : tagcode A} `{tcB : tagcode B}:
-  forall a b, Int.modu (@int_of_tag (A * B) (prod_tc tcA tcB) (a,b)) 
-                      (Int.repr (two_power_nat (tc_bitsize tcB))) =
+  forall a b, Int.modu (@int_of_tag (A * B) (tag_prod tcA tcB) (a,b)) 
+                      (Int.repr (two_power_nat (tag_bitsize tcB))) =
               int_of_tag b.
 Proof.
   intros.
   unfold int_of_tag. simpl.
-(* SearchAbout Int.modu. *)
+
+(*
+  remember (tag_bitsize tcB).
+  SearchAbout Int.modu.
+  rewrite Int.modu_divu.
+  SearchAbout Int.divu.
+  SearchAbout Int.sub.
+ *)
+  
 Admitted.
 
 Lemma int_of_tag_divu {A} {B} `{tcA : tagcode A} `{tcB : tagcode B}:
-  forall a b, Int.divu (@int_of_tag (A * B) (prod_tc tcA tcB) (a,b)) 
-                      (Int.repr (two_power_nat (tc_bitsize tcB))) =
+  forall a b, Int.divu (@int_of_tag (A * B) (tag_prod tcA tcB) (a,b)) 
+                      (Int.repr (two_power_nat (tag_bitsize tcB))) =
               int_of_tag a.
 Proof.
   intros.
   unfold int_of_tag. simpl.
-(* SearchAbout Int.divu. *)
-Admitted.
+
+(*  SearchAbout Int.divu. *)
+  Admitted.
