CertiGC/verif_gc.v
@@ -1,61 +1,194 @@
 Require Import VST.floyd.proofauto.
-Require Import RamifyCoq.CertiGC.env_gc. (* *)
 Require Import RamifyCoq.graph.graph_model.
 Require Import RamifyCoq.graph.path_lemmas.
 Require Import RamifyCoq.graph.subgraph2.
 Require Import RamifyCoq.graph.graph_relation.
 Require Import RamifyCoq.graph.reachable_computable.
 Require Import RamifyCoq.msl_application.Graph.
-Require Import RamifyCoq.CertiGC.GList. (* *)
-Require Import RamifyCoq.CertiGC.GList_GC. (* *)
 Require Import RamifyCoq.floyd_ext.share.
-Require Import RamifyCoq.CertiGC.spatial_graph_gc. (* *)
+Require Import RamifyCoq.graph.FiniteGraph.
+Require Import RamifyCoq.CertiGC.gc_mathgraph.
+Require Import RamifyCoq.CertiGC.env_gc. 
 
-Print GList.Graph.
 Local Open Scope logic.
 
-Arguments SingleFrame' {l} {g} {s}.
+Local Coercion pg_lg : LabeledGraph >-> PreGraph.
+Local Coercion lg_gg : GeneralGraph >-> LabeledGraph.
 
-Local Coercion Graph_LGraph: Graph >-> LGraph.
-Local Coercion LGraph_SGraph: LGraph >-> SGraph.
-Local Identity Coercion Graph_GeneralGraph: Graph >-> GeneralGraph.
-Local Identity Coercion LGraph_LabeledGraph: LGraph >-> LabeledGraph.
-Local Identity Coercion SGraph_SpatialGraph: SGraph >-> SpatialGraph.
-Local Coercion pg_lg: LabeledGraph >-> PreGraph.
+Definition V := val.
 
-Notation vertices_at sh P g:= (@vertices_at _ _ _ _ _ _ (@SGP pSGG_VST nat unit (sSGG_VST sh)) _ P g).
-Notation whole_graph sh g := (vertices_at sh (vvalid g) g).
-Notation graph sh x g := (@reachable_vertices_at _ _ _ _ _ _ _ _ _ _ (@SGP pSGG_VST nat unit (sSGG_VST sh)) _ x g).
-Notation Graph := (@Graph pSGG_VST nat unit unit).
-Existing Instances maGraph finGraph liGraph RGF.
+Parameter DV : Type.
+Parameter DE : Type.
+Parameter DG : Type.
 
+Definition max_spaces : nat := 10.
+
+Definition reachable_through_vertices_at (S: list addr) (g: env_Graph): mpred :=
+  @vertices_at addr E _ _
+               SGBA_GCgraph
+               mpred
+               (@SGP_VST fullshare g) 
+               (@SGA_VST fullshare g) 
+               (@reachable_through_set addr E _ _ g S)
+              (@Graph_PointwiseGraph addr E _ _ (@SGBA_GCgraph addr _) LV LE LG (SGC_GCgraph) (lg_gg g)).
+
+Definition gc_graph_pred (roots : list addr) (g : env_Graph) :=
+  reachable_through_vertices_at roots g.
+
+Local Open Scope nat_scope.
+
+Fixpoint get_roots_helper n indices args : list addr :=
+  match n with
+  | 0 => []
+  | _ => match indices with
+        | [] => [] (* bad news *)
+        | h :: t => (List.nth h args NullPointer) :: get_roots_helper (n-1) t args
+        end
+  end.
+
+(* 
+This is oversimplified. 
+I actually need to take ti, a Tstruct of type _thread_info, and learn how to get the args array myself. 
+*)
+Definition get_roots (fi : list nat) (args : list addr) : list addr :=
+  match fi with
+  | _ :: n :: t => get_roots_helper n t args
+  | _ => [] (* bad news *)
+  end.
+
+(* 
+Questions:
+1. can I just take a space, and then get the parameters from inside the space and then hook up those parameters to the function arguments when linking in PRE?
+*)
+Definition forward_spec :=
+ DECLARE _forward
+  WITH 	sh: wshare, 
+  	g: env_Graph, 
+  	start: pointer_val, 
+  	limit: pointer_val, 
+  	next: pointer_val, 
+  	p: pointer_val,
+        depth : nat,
+        gen : nat, (* implicit, thanks to the caller *)
+        roots_locs: list pointer_val 
+                               
+  PRE [ _from_start OF tptr (Tlong Unsigned noattr),
+  	_from_limit OF tptr (Tlong Unsigned noattr),
+  	_next OF tptr (tptr (Tlong Unsigned noattr)),
+  	_p OF tptr (Tlong Unsigned noattr) ]
+  EX roots,
+    PROP (cleared_for_forward g gen start next limit p) (* Props of Coq type Prop, describing things that are forever true *)
+    LOCAL ( temp _from_start (pointer_val_val start); 
+  	    temp _from_limit (pointer_val_val limit);
+  	    temp _next (pointer_val_val next);(* *)
+  	    temp _p (pointer_val_val p) )
+  	SEP (tarray roots_locs roots * graph_pred g roots) 
+  POST [Tvoid]
+  EX g' : Graph,
+  EX roots,
+
+          EX v: pointer_val, EX v': pointer_val, (* also, gen : nat *)
+        PROP ()
+(*((~(vvalid g \/) -> g = g' ) /\ (* etc *)
+  	       ~ in_from g gen v \/ (* slightly off (re: quantifiers) *)
+  	       (* "already copied" - adding a case to stepish *)
+  	       (* update: seems there is no need; copyitem may cover it. *)
+  	      copyitem g g' gen v v')*)
+               (* strengthen stepish? *)
+  	LOCAL ()
+  	SEP (graph_pred g' roots).
+
+
+
+
+Definition forward_roots_spec :=
+ DECLARE _forward_roots
+  WITH  sh: wshare,
+        g: raw_GCgraph,
+        start: pointer_val,
+        limit: pointer_val,   
+        next: pointer_val, 
+        fi: pointer_val (* ?? *),
+        ti: pointer_val (* ?? *)
+  PRE [ _from_start OF tptr (Tlong Unsigned noattr),
+        _from_limit OF tptr (Tlong Unsigned noattr),
+        _next OF tptr (tptr (Tlong Unsigned noattr)),
+        _fi OF tptr (Tlong Unsigned noattr),
+        _ti OF tptr (Tstruct _thread_info noattr)]
+    PROP () (* props of Coq type Prop, describing things that are forever true *) 
+    LOCAL ( temp _from_start (pointer_val_val start); 
+            temp _from_limit (pointer_val_val limit);
+            temp _next (pointer_val_val next);
+            temp _ti (pointer_val_val ti);
+            temp _fi (pointer_val_val fi) )
+    SEP (GC_graph g)
+  POST [Tvoid]
+    EX g' : raw_GCgraph, (* gen : nat *)
+    PROP ()
+          (* need the double indirection here
+               want to say forward with a forall over the args array
+            *)
+    LOCAL ()
+    SEP (GC_graph g /\ GC_graph g').
+
+(*
+void garbage_collect(fun_info fi, struct thread_info *ti)
+ *)
+
+(* need to fix fi's type. pointer_val is for c pointers *)
+(* worth noting that fi is a unintnat* pointer *)
+(* there are drastically different PRE and POST conditions depending on whether the heap was already created. how to encode? *)
+(* whole_graph_valid seems like something I can borrow from Shengyi. *)
 Definition garbage_collect_spec :=
   DECLARE _garbage_collect 
-  WITH sh: wshare, fi : pointer_val, ti : pointer_val
+  WITH sh: wshare, g: env_Graph, fi : pointer_val (*???*), ti : pointer_val
   PRE [_fi OF (tptr tuint ), _ti OF (tptr (Tstruct _thread_info noattr))]
-     PROP ()
-     LOCAL (temp _fi (pointer_val_val fi); temp _ti (pointer_val_val ti))
-     SEP ()
+     PROP (whole_graph_valid g fi ti)
+     LOCAL (temp _fi (pointer_val_val (*???*) fi); temp _ti (pointer_val_val ti))
+     SEP (whole_graph sh g)
   POST [ tptr tvoid ]
-     PROP ()
+  PROP (whole_graph_valid g' fi ti /\
+        iso_from_roots g g' fi ti /\
+        points_to_unalloc (*next ptr*))
      LOCAL ()
-     SEP ().
+     SEP (whole_graph sh g').
 
+(*
+Definition whole_graph sh g x := (@full_graph_at mpred SAGA_VST pointer_val (SAG_VST sh) g x).
+ *)
+
+
+(* POSSIBLE HINT: do_generation basically calls forward_roots, then do_scan, and then aborts. the specs should be intimately related. *)
+(* nextIsStart just says ``from->next=from->start'' *)
+(* there are two complex postconditions that are basically specs of their own *)
 Definition do_generation_spec :=
   DECLARE _do_generation 
-  WITH sh: wshare, from : val, to : val, fi : val, ti : val
-     PRE [ _from OF (tptr (Tstruct _space noattr)),
-           _to OF (tptr (Tstruct _space noattr)),
-           _fi OF (tptr tuint),
-           _ti OF (tptr (Tstruct _thread_info noattr))]
-     PROP ()
+  WITH sh: wshare, from : val, to : val, fi : ???, ti : val
+     PRE [ temp _from OF (tptr (Tstruct _space noattr)),
+           temp _to OF (tptr (Tstruct _space noattr)),
+           temp _fi OF (tptr tuint),
+           temp _ti OF (tptr (Tstruct _thread_info noattr))]
+     PROP (some_form_of_validity g fi ti /\
+           from_is_full g fi ti /\
+           to_has_room g fi ti)
      LOCAL (temp _from from; temp _to to; temp _fi fi; temp _ti ti)
-     SEP ()
+     SEP (whole_graph sh g)
   POST [ tptr tvoid ]
-     PROP ()
+     EX g' : Graph, args' : ???, (* this will probably be a `` ti' '' instead. *)
+                                 (* the new args will live inside the new ti *)    
+     PROP (whole_graph sh g /\
+          nextIsStart from /\
+          ??? /\ ???)
+     (* instead of writing this out, I want to reuse the specs for forward_roots and do_scan. Shengyi doesn't know how, but he did give me the hint above. Hmm. *)
      LOCAL ()
-     SEP ().
+     SEP (whole_graph g /\ whole_graph g').
 
+(* 
+void do_scan(value *from_start,  /* beginning of from-space */
+	     value *from_limit,  /* end of from-space */
+	     value *scan,        /* start of unforwarded part of to-space */
+ 	     value **next)       /* next available spot in to-space */
+*)
 Definition do_scan_spec :=
   DECLARE _do_scan 
   WITH sh: wshare, start : val, limit : val, scan : val, next : val
@@ -63,18 +196,23 @@ Definition do_scan_spec :=
            _from_limit OF (tptr tint),
            _scan OF (tptr tint),
            _next OF (tptr (tptr tint))]
-     PROP ()
+     PROP (no_pointers_from (*to_start*) (*to_scan*) (*from_start*) (*from_limit*))
      LOCAL (temp _from_start start; temp _from_limit limit;
             temp _scan scan; temp _next next)  
      SEP ()
   POST [ tptr tvoid ]
-     PROP ()
+  PROP (subgraphs_iso g g' fi ti /\
+        (* want to say that only to and from were even touched *) /\
+        (* to->scan' == to->next'
+	to->scan' ≥ to->scan 
+	to->next' ≥ to->next *) /\
+        no_pointers_from (*to_start*) (*to_next'*) (*from_start*) (*from_limit*))
      LOCAL ()
      SEP ().
 
 Definition forward_roots_spec :=
   DECLARE _forward_roots 
-  WITH sh: wshare, start : val, limit : val, ti : val, fi : val, next : val
+  WITH sh: wshare, start : val, limit : val, ti : val, fi : ??, next : val
      PRE [ _from_start OF (tptr tint),
            _from_limit OF (tptr tint),
            _next OF (tptr (tptr tint)),
@@ -85,26 +223,13 @@ Definition forward_roots_spec :=
             temp _next next; temp _fi fi; temp _ti ti)
      SEP ()
   POST [ tptr tvoid ]
-     PROP ()
+  PROP (subgraphs_iso g g' fi ti /\
+       (* to->next' ≥ to->next *) /\ 
+        no_pointers_from  (*live roots slots of the args array *) (*from_start*) (*from_limit*))
      LOCAL ()
      SEP ().
-     
-Definition forward_spec :=
-  DECLARE _forward 
-  WITH sh: wshare, start : val, limit : val, next : val, p : val, depth : val
-     PRE [ _from_start OF (tptr tint),
-           _from_limit OF (tptr tint),
-           _next OF (tptr (tptr tint)),
-           _p OF (tptr tint),
-           _depth OF (tint)]
-     PROP ()
-     LOCAL (temp _from_start start; temp _from_limit limit;
-            temp _next next; temp _p p; temp _depth depth)
-     SEP ()
-  POST [ tptr tvoid ]
-     PROP ()
-     LOCAL ()
-     SEP ().
+
+
 
 (***********************)
 (** below is UF stuff **)
